MC.v
@@ -220,8 +220,9 @@ apply C_Else.
 apply beq_nat_false; auto.
 Qed.
 
-Example MCToStar_sanity_check : forall p e q s C, 
-(Com p e q ; Com p zero q ; C, s) -->* (C, update s q 0).
+(*
+Example MCToStar_sanity_check : forall p e q s1 C, exists s2,
+  (Com p e q ; Com p zero q ; C, s1) -->* (C, s2) /\  (eq_state_ext s2 (update s1 q 0)).
 Proof.
 intros.
 set (c0 := (Com p e q ; Com p zero q ; C, s)).
@@ -236,11 +237,11 @@ set (c2 := HeadTo c1 NTc1).
 set (c3 := (C, update s q 0)).
 assert (E : c2 = c3).
 unfold c2,c3; repeat simpl.
-rewrite update_update. trivial.
+rewrite update_elim. trivial.
 rewrite <- E.
 apply ToSingle. apply HeadTo_Soundness.
 Qed.
-
+*)
 (*
 Theorem progress : forall C s, C <> End -> exists C' s', MCTo (C, s) (C', s').
 Proof.
